
---
title: 独立事件
tag: [](./index.md)
asref: true
---

$\gdef\spaces#1{~ #1 ~}$

以下命题均为事件相互独立的充要条件

1. $P(AB) = P(A)P(B)$

1. $P(A|B) = P(A)$ \
    $\qquad \iff P(A|\overline B) = P(A)$ \
    $\qquad \iff P(A|B) = P(A|\overline B)$, $0 < P(B) < 1$

1. $A$ 与 $\overline B$ 或 $B$ 与 $\overline A$ 或 $\overline A$ 或 $\overline B$ 相互独立

1. $P(A|B) + P(\overline A | \overline B) = 1$ \
    $\qquad \iff P(A|\overline{B}) + P(\overline{A}|B) = 1$, $0 < P(B) < 1$


这里 $(2) \implies (1)$ 是因为 $P(A|B)P(B) = P(AB) = P(B|A)P(A)$, 此时如果再用 $P(A|B) = P(A)$, 立刻就有 $P(A)P(B) = P(AB)$. 

对于 $(4)$, 我们只展示 $0 < P(B) < 1$ 时有 $P(A|\overline{B}) + P(\overline{A}|B) = 1 \iff P(AB) = P(A)P(B)$. 另一个等式的验证是类似的. 因为 

$$
\begin{aligned}
P(A|\overline{B}) + P(\overline{A}|B) 
&\spaces= \frac{P(A\overline{B})}{P(\overline B)} + \frac{P(\overline{A}B)}{P(B)} \\
&\spaces= \frac{P(A) - P(AB)}{1-P(B)} + \frac{P(B) - P(AB)}{P(B)} \\
&\spaces= 1
\end{aligned}
$$

全展开得 $P(A)P(B) {\color{8a58ed} - P(AB)P(B) } + {\color{32a852} P(B) - P(B)^2} - P(AB) {\color{8a58ed} + P(AB)P(B)} = {\color{32a852} P(B) - P(B)^2}$. 即 $P(A)P(B) = P(AB)$.  
